erasure/theories/EGlobalEnv.v
@@ -49,6 +49,13 @@ Qed.
 Section Lookups.
   Context (Σ : global_declarations).
 
+  Definition lookup_constant kn : option constant_body :=
+    decl <- lookup_env Σ kn;; 
+    match decl with
+    | ConstantDecl cdecl => ret cdecl
+    | InductiveDecl mdecl => None
+    end.
+
   Definition lookup_minductive kn : option mutual_inductive_body :=
     decl <- lookup_env Σ kn;; 
     match decl with
@@ -65,9 +72,13 @@ Section Lookups.
     mdecl <- lookup_minductive kn ;;
     ret mdecl.(ind_npars).
   
-  Definition lookup_constructor_pars_args kn c : option (nat * nat) := 
+  Definition lookup_constructor kn c : option (mutual_inductive_body * one_inductive_body * (ident * nat)) :=
     '(mdecl, idecl) <- lookup_inductive kn ;;
     cdecl <- nth_error idecl.(ind_ctors) c ;;
+    ret (mdecl, idecl, cdecl).
+  
+  Definition lookup_constructor_pars_args kn c : option (nat * nat) := 
+    '(mdecl, idecl, cdecl) <- lookup_constructor kn c ;;
     ret (mdecl.(ind_npars), cdecl.2).
 End Lookups.
 
@@ -100,14 +111,6 @@ Definition extends (Σ Σ' : global_declarations) := ∑ Σ'', Σ' = (Σ'' ++ Σ
 Definition fresh_global kn (Σ : global_declarations) :=
   Forall (fun x => x.1 <> kn) Σ.
 
-Inductive wf_glob : global_declarations -> Prop :=
-| wf_glob_nil : wf_glob []
-| wf_glob_cons kn d Σ : 
-  wf_glob Σ ->
-  fresh_global kn Σ ->
-  wf_glob ((kn, d) :: Σ).
-Derive Signature for wf_glob.
-
 Lemma lookup_env_Some_fresh {Σ c decl} :
   lookup_env Σ c = Some decl -> ~ (fresh_global c Σ).
 Proof.
@@ -119,32 +122,6 @@ Proof.
     now inv H2.
 Qed.
 
-Lemma extends_lookup {Σ Σ' c decl} :
-  wf_glob Σ' ->
-  extends Σ Σ' ->
-  lookup_env Σ c = Some decl ->
-  lookup_env Σ' c = Some decl.
-Proof.
-  intros wfΣ' [Σ'' ->]. simpl.
-  induction Σ'' in wfΣ', c, decl |- *.
-  - simpl. auto.
-  - specialize (IHΣ'' c decl). forward IHΣ''.
-    + now inv wfΣ'.
-    + intros HΣ. specialize (IHΣ'' HΣ).
-      inv wfΣ'. simpl in *.
-      case: eqb_spec; intros e; subst; auto.
-      apply lookup_env_Some_fresh in IHΣ''; contradiction.
-Qed.
-
-Lemma extends_is_propositional {Σ Σ'} : 
-  wf_glob Σ' -> extends Σ Σ' ->
-  forall ind b, inductive_isprop_and_pars Σ ind = Some b -> inductive_isprop_and_pars Σ' ind = Some b.
-Proof.
-  intros wf ex ind b.
-  rewrite /inductive_isprop_and_pars.
-  destruct lookup_env eqn:lookup => //.
-  now rewrite (extends_lookup wf ex lookup).
-Qed.
 
 (** ** Reduction *)
 
@@ -212,10 +189,14 @@ Definition tDummy := tVar "".
 Definition iota_red npar args (br : list name * term) :=
   substl (List.rev (List.skipn npar args)) br.2.
 
+Definition isSome {A} (o : option A) := 
+  match o with 
+  | None => false
+  | Some _ => true
+  end.
 
-  Class switchterm := 
-  { 
-  has_tBox : bool
+Class ETermFlags := 
+  { has_tBox : bool
   ; has_tRel : bool
   ; has_tVar : bool
   ; has_tEvar : bool
@@ -229,11 +210,36 @@ Definition iota_red npar args (br : list name * term) :=
   ; has_tFix : bool
   ; has_tCoFix : bool
   }.
+
+Class EEnvFlags := {
+  has_axioms : bool;
+  has_cstr_params : bool;
+  term_switches :> ETermFlags }.
   
+Definition all_term_flags := 
+  {| has_tBox := true
+    ; has_tRel := true
+    ; has_tVar := true
+    ; has_tEvar := true
+    ; has_tLambda := true
+    ; has_tLetIn := true
+    ; has_tApp := true
+    ; has_tConst := true
+    ; has_tConstruct := true
+    ; has_tCase := true
+    ; has_tProj := true
+    ; has_tFix := true
+    ; has_tCoFix := true
+  |}.
+
+Definition all_env_flags := 
+  {| has_axioms := true; 
+     term_switches := all_term_flags;
+     has_cstr_params := true |}.
+    
 Section wf.
   
-  Context {sw  : switchterm}.
-  Variable has_axioms : bool.
+  Context {sw  : EEnvFlags}.
   Variable Σ : global_context.
 
   (* a term term is wellformed if
@@ -252,8 +258,8 @@ Section wf.
     | tLetIn na b b' => has_tLetIn && wellformed k b && wellformed (S k) b'
     | tCase ind c brs => has_tCase && 
       let brs' := List.forallb (fun br => wellformed (#|br.1| + k) br.2) brs in
-      wellformed k c && brs'
-    | tProj p c => has_tProj && wellformed k c
+      isSome (lookup_inductive Σ ind.1) && wellformed k c && brs'
+    | tProj p c => has_tProj && isSome (lookup_inductive Σ p.1.1) && wellformed k c
     | tFix mfix idx => has_tFix &&
       let k' := List.length mfix + k in
       List.forallb (test_def (wellformed k')) mfix
@@ -261,19 +267,58 @@ Section wf.
       let k' := List.length mfix + k in
       List.forallb (test_def (wellformed k')) mfix
     | tBox => has_tBox
-    | tConst kn => has_tConst && match lookup_env Σ kn with Some (ConstantDecl d) => 
-        has_axioms || match d.(cst_body) with Some _ => true | _ => false end 
-        | _ => false end
-    | tConstruct ind c => has_tConstruct &&
-        match lookup_env Σ ind.(inductive_mind) with 
-        | Some (InductiveDecl mdecl) => 
-          match nth_error (ind_bodies mdecl) (inductive_ind ind) with 
-          | Some idecl => match nth_error (ind_ctors idecl) c with Some _ => true | _ => false end
-          | _ => false
-          end
-        | _ => false
-        end    
+    | tConst kn => has_tConst && 
+      match lookup_constant Σ kn with
+      | Some d => has_axioms || isSome d.(cst_body)
+      | _ => false 
+      end
+    | tConstruct ind c => has_tConstruct && isSome (lookup_constructor Σ ind c)
     | tVar _ => has_tVar
     end.
 
 End wf.
+
+Definition wf_global_decl {sw : EEnvFlags} Σ d : bool :=
+  match d with
+  | ConstantDecl cb => option_default (fun b => wellformed Σ 0 b) cb.(cst_body) has_axioms
+  | InductiveDecl idecl => has_cstr_params || (idecl.(ind_npars) == 0)
+  end.
+
+Inductive wf_glob {efl : EEnvFlags} : global_declarations -> Prop :=
+| wf_glob_nil : wf_glob []
+| wf_glob_cons kn d Σ : 
+  wf_glob Σ ->
+  wf_global_decl Σ d ->
+  fresh_global kn Σ ->
+  wf_glob ((kn, d) :: Σ).
+Derive Signature for wf_glob.
+
+Implicit Types (efl : EEnvFlags).
+
+Lemma extends_lookup {efl} {Σ Σ' c decl} :
+  wf_glob Σ' ->
+  extends Σ Σ' ->
+  lookup_env Σ c = Some decl ->
+  lookup_env Σ' c = Some decl.
+Proof.
+  intros wfΣ' [Σ'' ->]. simpl.
+  induction Σ'' in wfΣ', c, decl |- *.
+  - simpl. auto.
+  - specialize (IHΣ'' c decl). forward IHΣ''.
+    + now inv wfΣ'.
+    + intros HΣ. specialize (IHΣ'' HΣ).
+      inv wfΣ'. simpl in *.
+      case: eqb_spec; intros e; subst; auto.
+      apply lookup_env_Some_fresh in IHΣ''; contradiction.
+Qed.
+
+Lemma extends_is_propositional {efl} {Σ Σ'} : 
+  wf_glob Σ' -> extends Σ Σ' ->
+  forall ind b, inductive_isprop_and_pars Σ ind = Some b -> inductive_isprop_and_pars Σ' ind = Some b.
+Proof.
+  intros wf ex ind b.
+  rewrite /inductive_isprop_and_pars.
+  destruct lookup_env eqn:lookup => //.
+  now rewrite (extends_lookup wf ex lookup).
+Qed.
+
